WIP on IPv4 derivation.

src/BinEncoders/Env/Examples/IPv4Header.v
@@ -4,6 +4,7 @@ Require Import
 
 Require Import
         Fiat.Common.SumType
+        Fiat.Common.EnumType
         Fiat.Common.BoundedLookup
         Fiat.Common.ilist
         Fiat.Computation
@@ -20,6 +21,7 @@ Require Import
         Fiat.BinEncoders.Env.Lib2.FixListOpt
         Fiat.BinEncoders.Env.Lib2.NoCache
         Fiat.BinEncoders.Env.Lib2.WordOpt
+        Fiat.BinEncoders.Env.Lib2.Bool
         Fiat.BinEncoders.Env.Lib2.NatOpt
         Fiat.BinEncoders.Env.Lib2.Vector
         Fiat.BinEncoders.Env.Lib2.EnumOpt
@@ -39,7 +41,7 @@ Definition IPv4_Packet :=
           "MF" :: bool, (*  Multiple fragments flag *)
           "FragmentOffset" :: word 13,
           "TTL" :: char,
-          "Protocol" :: BoundedString ["ICMP"; "TCP"; "UDP"],
+          "Protocol" :: EnumType ["ICMP"; "TCP"; "UDP"],
           (* So many to choose from: http://www.iana.org/assignments/protocol-numbers/protocol-numbers.xhtml*)
           "SourceAddress" :: word 32,
           "DestAddress" :: word 32,
@@ -55,17 +57,300 @@ Variable IPChecksum : ByteString -> ByteString.
 
 Definition transformer : Transformer ByteString := ByteStringTransformer.
 
-Definition encode_IPv4_Packet_Spec (ip4 : IPv4_Packet) (payload_len : nat) :=
-          encode_word_Spec (natToWord 4 4)
+Definition encode_IPv4_Packet_Spec (ip4 : IPv4_Packet)  :=
+          (encode_word_Spec (natToWord 4 4)
     ThenC encode_nat_Spec 4 (5 + |ip4!"Options"|)
-    ThenC encode_nat_Spec 4 (5 + |ip4!"Options"| + payload_len) (* payload length is an argument *)
+    ThenC encode_unused_word_Spec 8 (* TOS Field! *)
+    ThenC (fun ctx => payload_len <- {payload_len : nat | lt (20 + (4 * |ip4!"Options"|) + payload_len) (pow2 16)};
+             encode_nat_Spec 16 (20 + (4 * |ip4!"Options"|) + payload_len) ctx) (* payload length is an argument *)
     ThenC encode_word_Spec ip4!"ID"
-    ThenC (Either encode_word_Spec WO~1 Or encode_word_Spec WO~0) (* Unused flag! *)
-    ThenC encode_word_Spec (WS ip4!"DF" WO)
-    ThenC encode_word_Spec (WS ip4!"MF" WO)
+    ThenC encode_unused_word_Spec 1 (* Unused flag! *)
+    ThenC encode_bool_Spec ip4!"DF"
+    ThenC encode_bool_Spec ip4!"MF"
     ThenC encode_word_Spec ip4!"FragmentOffset"
     ThenC encode_word_Spec ip4!"TTL"
+    ThenC encode_enum_Spec ProtocolTypeCodes ip4!"Protocol"
+    DoneC)
     ThenChecksum IPChecksum
-    ThenCarryOn encode_word_Spec ip4!"SourceAddress"
+    ThenCarryOn (encode_word_Spec ip4!"SourceAddress"
     ThenC encode_word_Spec ip4!"DestAddress"
-    ThenC encode_list_Spec encode_word_Spec ip4!"Options".
+    ThenC encode_list_Spec encode_word_Spec ip4!"Options"
+    DoneC).
+
+Definition IPv4_Packet_OK (ipv4 : IPv4_Packet) :=
+  lt (|ipv4!"Options"|) 11.
+
+Variable IPChecksum_Valid : nat -> ByteString -> Prop.
+Variable IPChecksum_Valid_dec : forall n b, {IPChecksum_Valid n b} + {~IPChecksum_Valid n b}.
+Variable decodeChecksum : ByteString -> CacheDecode -> option (() * ByteString * CacheDecode).
+
+Variable IPChecksum_OK : forall b ext : ByteString, IPChecksum_Valid (bin_measure (transform b (IPChecksum b))) (transform (transform b (IPChecksum b)) ext).
+
+Variable IPChecksum_commute : forall b b' : ByteString, IPChecksum (transform b b') = IPChecksum (transform b' b).
+
+Variable IPChecksum_Valid_commute :
+  forall b b' ext : ByteString,
+    IPChecksum_Valid (bin_measure (transform b b')) (transform (transform b b') ext) <-> IPChecksum_Valid (bin_measure (transform b' b)) (transform (transform b' b) ext).
+
+Variable IPv4_Packet_encoded_measure  : ByteString -> nat.
+
+Lemma IPv4_Packet_encoded_measure_OK :
+  forall (a : IPv4_Packet) (ctx ctx' : ()) (b ext : ByteString),
+    encode_IPv4_Packet_Spec a ctx ↝ (b, ctx')
+    -> length_ByteString b = IPv4_Packet_encoded_measure (ByteString_transformer b ext).
+Admitted.
+
+Lemma decodeIPChecksum_pf
+  : forall (b b' ext : ByteString) (ctx ctx' ctxD : ()),
+    True ->
+    decodeChecksum (ByteString_transformer (ByteString_transformer (IPChecksum (ByteString_transformer b b')) b') ext) ctxD = Some ((), ByteString_transformer b' ext, ctxD).
+Admitted.
+
+Lemma decodeIPChecksum_pf'
+  : forall (u : ()) (b b' : ByteString),
+    () -> forall ctxD ctxD' : (), True -> decodeChecksum b ctxD = Some (u, b', ctxD') -> True /\ (exists b'' : ByteString, b = ByteString_transformer b'' b').
+Proof.
+Admitted.
+
+Transparent pow2.
+Arguments pow2 : simpl never.
+
+Definition EthernetHeader_decoder
+  : { decodePlusCacheInv |
+      exists P_inv,
+        (cache_inv_Property (snd decodePlusCacheInv) P_inv
+         -> encode_decode_correct_f _ transformer IPv4_Packet_OK (fun _ _ => True)
+                                    encode_IPv4_Packet_Spec
+                                    (fst decodePlusCacheInv) (snd decodePlusCacheInv))
+        /\ cache_inv_Property (snd decodePlusCacheInv) P_inv}.
+Proof.
+  eexists (_, _); intros; eexists _; split; simpl.
+  intros.
+  unfold encode_IPv4_Packet_Spec; pose_string_ids.
+  eapply (@composeChecksum_encode_correct
+              IPv4_Packet _ transformer IPChecksum
+              IPChecksum_Valid IPChecksum_Valid_dec
+              IPChecksum_OK IPChecksum_commute IPChecksum_Valid_commute _
+              (nat * (word 16 * (bool * (bool * (word 13 * (char * EnumType ["ICMP"; "TCP"; "UDP"]))))))
+              _ _ _ decodeChecksum H
+              (fun ip4 => (|ip4!StringId10|, (ip4!StringId, (ip4!StringId0,
+                           (ip4!StringId1, (ip4!StringId2, (ip4!StringId3, ip4!StringId4)))))))
+              (IPv4_Packet_OK)
+              _ _ _
+              (fun data' : nat * (word 16 * (bool * (bool * (word 13 * (char * EnumType ["ICMP"; "TCP"; "UDP"]))))) =>
+                 (encode_word_Spec (natToWord 4 4)
+                                   ThenC encode_nat_Spec 4 (5 + fst data')
+                                   ThenC encode_unused_word_Spec 8 (* TOS Field! *)
+                                   ThenC (fun ctx => payload_len <- {payload_len : nat | lt (20 + (4 * (fst data')) + payload_len) (pow2 16)};
+             encode_nat_Spec 16 (20 + (4 * (fst data')) + payload_len) ctx)
+                                   ThenC encode_word_Spec (fst (snd data'))
+                                   ThenC encode_unused_word_Spec 1
+                                   ThenC encode_bool_Spec (fst (snd (snd data')))
+                                   ThenC encode_bool_Spec (fst (snd (snd (snd data'))))
+                                   ThenC encode_word_Spec (fst (snd (snd (snd (snd data')))))
+                                   ThenC encode_word_Spec (fst (snd (snd (snd (snd (snd data'))))))
+                                   ThenC encode_enum_Spec ProtocolTypeCodes (snd (snd (snd (snd (snd (snd data'))))))
+                                   DoneC)));
+    simpl.
+  intros; eapply IPv4_Packet_encoded_measure_OK; apply H0.
+  apply_compose.
+  eapply Word_decode_correct.
+  solve_data_inv.
+  solve_data_inv.
+  apply_compose.
+  eapply Nat_decode_correct.
+  solve_data_inv.
+  solve_data_inv.
+  unfold encode_unused_word_Spec.
+  apply_compose.
+  eapply unused_word_decode_correct.
+  solve_data_inv.
+  solve_data_inv.
+  simpl.
+  apply_compose.
+  eapply Nat_decode_correct.
+  solve_data_inv.
+  solve_data_inv.
+  apply_compose.
+  eapply Word_decode_correct.
+  solve_data_inv.
+  solve_data_inv.
+  apply_compose.
+  eapply unused_word_decode_correct.
+  solve_data_inv.
+  solve_data_inv.
+  apply_compose.
+  eapply bool_decode_correct.
+  solve_data_inv.
+  solve_data_inv.
+  apply_compose.
+  eapply bool_decode_correct.
+  solve_data_inv.
+  solve_data_inv.
+  apply_compose.
+  eapply Word_decode_correct.
+  solve_data_inv.
+  solve_data_inv.
+  apply_compose.
+  eapply Word_decode_correct.
+  solve_data_inv.
+  solve_data_inv.
+  apply_compose.
+  eapply Enum_decode_correct.
+  Discharge_NoDupVector.
+  solve_data_inv.
+  solve_data_inv.
+  unfold encode_decode_correct_f; intuition eauto.
+  instantiate
+    (1 := fun p b env => if Compare_dec.le_lt_dec proj 4 then None else _ p b env).
+  simpl in *.
+  rewrite <- H24; simpl.
+  assert (a = proj - 5) by
+      (rewrite <- H24; simpl; auto with arith).
+  clear H24.
+  computes_to_inv; injections; subst; simpl.
+  pose proof transform_id_left as H'; simpl in H'; rewrite H'.
+  eexists env'; simpl; intuition eauto.
+  instantiate (1 := fun proj6 ext env' => Some (proj - 5, (proj1, (proj2, (proj3, (proj4, (proj5, proj6))))), ext, env')).
+  simpl; rewrite <- Minus.minus_n_O; reflexivity.
+  find_if_inside; try discriminate.
+  simpl in H14; injections; eauto.
+  simpl in H14; repeat find_if_inside; try discriminate.
+  injections.
+  simpl.
+  eexists _; eexists tt;
+    intuition eauto; injections; eauto using idx_ibound_eq;
+      try match goal with
+            |-  ?data => destruct data;
+                           simpl in *; eauto
+          end.
+  destruct env; computes_to_econstructor.
+  pose proof transform_id_left as H'; simpl in H'; rewrite H'.
+  reflexivity.
+  instantiate (1 := fun _ => True); simpl; eauto.
+  revert H1 l payload_OK; clear; intros;
+  unfold pow2 in H1; simpl in H1.
+  omega.
+  revert H1 l; unfold pow2; simpl; intros; omega.
+  revert H1 l; unfold pow2; simpl; intros; omega.
+  simpl.
+  revert H1 l payload_OK; clear; intros;
+  unfold pow2 in H1; simpl in H1.
+  omega.
+  unfold IPv4_Packet_OK; intros; destruct H0; repeat split; eauto.
+  simpl.
+  unfold StringId10.
+  unfold pow2; simpl.
+  match goal with
+    |- context [length ?x] =>
+    revert H0; simpl; remember (length x); clear;
+      auto with arith
+  end.
+  instantiate (1 := fun _ _ => True);
+    simpl; intros; exact I.
+  intros; eapply decodeIPChecksum_pf; eauto.
+  intros; eapply decodeIPChecksum_pf'; eauto.
+  apply_compose.
+  eapply Word_decode_correct.
+  solve_data_inv.
+  solve_data_inv.
+  apply_compose.
+  eapply Word_decode_correct.
+  solve_data_inv.
+  solve_data_inv.
+  apply_compose.
+  intro; eapply FixList_decode_correct.
+  revert H3; eapply Word_decode_correct.
+  simpl in *; split.
+  intuition eauto.
+  pose proof (f_equal fst H9).
+  simpl in H4; apply H4.
+  simpl in *; injections.
+  simpl; auto with arith.
+  eauto.
+  simpl; intros; eauto using FixedList_predicate_rest_True.
+  simpl; intros;
+    unfold encode_decode_correct_f; intuition eauto.
+  destruct data as [? [? [? [? [? [? [? [? [? [ ] ] ] ] ] ] ] ] ] ];
+    unfold GetAttribute, GetAttributeRaw in *;
+    simpl in *.
+  pose proof (f_equal fst H14).
+  pose proof (f_equal (fun z => fst (snd z)) H14).
+  pose proof (f_equal (fun z => fst (snd (snd z))) H14).
+  pose proof (f_equal (fun z => fst (snd (snd (snd z)))) H14).
+  pose proof (f_equal (fun z => fst (snd (snd (snd (snd z))))) H14).
+  pose proof (f_equal (fun z => fst (snd (snd (snd (snd (snd z)))))) H14).
+  pose proof (f_equal (fun z => fst (snd (snd (snd (snd (snd (snd z))))))) H14).
+  pose proof (f_equal (fun z => snd (snd (snd (snd (snd (snd (snd z))))))) H14).
+  simpl in *.
+  clear H14.
+  computes_to_inv; injections; subst; simpl.
+  pose proof transform_id_left as H'; simpl in H'; rewrite H'.
+  eexists env'; simpl; intuition eauto.
+  simpl in *.
+  simpl in H8; injections; eauto.
+  simpl in H8; repeat find_if_inside; try discriminate.
+  eexists _; eexists tt.
+  injections; simpl in *; repeat split.
+  destruct env; computes_to_econstructor.
+  pose proof transform_id_left as H'; simpl in H'; rewrite H'.
+  reflexivity.
+  unfold GetAttribute, GetAttributeRaw; simpl.
+  rewrite H5; eauto.
+  intuition.
+  simpl in *.
+  unfold pow2 in H9; simpl in H9; auto with arith.
+  omega.
+  unfold GetAttribute, GetAttributeRaw.
+  simpl.
+  rewrite H5.
+  revert payload_OK H0; clear; simpl.
+  intros; destruct H0 as [ [? ?] ?].
+  unfold pow2 in H1; simpl in H1.
+  omega.
+  destruct proj as [? [? [? [? [? [? [? ?] ] ] ] ] ] ].
+  simpl.
+  unfold GetAttribute, GetAttributeRaw; simpl in *.
+  repeat f_equal.
+  eauto.
+  rewrite H5; simpl.
+
+  apply_compose.
+  eapply Enum_decode_correct.
+  Discharge_NoDupVector.
+  solve_data_inv.
+  simpl; intros; exact I.
+  simpl; intros.
+  unfold encode_decode_correct_f; intuition eauto.
+  destruct data as [? [? [? [ ] ] ] ];
+    unfold GetAttribute, GetAttributeRaw in *;
+    simpl in *.
+  computes_to_inv; injections; subst; simpl.
+  pose proof transform_id_left as H'; simpl in H'; rewrite H'.
+  eexists env'; simpl; intuition eauto.
+  match goal with
+    |- ?f ?a ?b ?c = ?P =>
+    let P' := (eval pattern a, b, c in P) in
+    let f' := match P' with ?f a b c => f end in
+    try unify f f'; try reflexivity
+  end.
+  simpl in *; injections; eauto.
+  simpl in *; repeat find_if_inside; try discriminate.
+  eexists _; eexists tt;
+    intuition eauto; injections; eauto using idx_ibound_eq;
+      try match goal with
+            |-  ?data => destruct data;
+                           simpl in *; eauto
+          end.
+  destruct env; computes_to_econstructor.
+  pose proof transform_id_left as H'; simpl in H'; rewrite H'.
+  reflexivity.
+  repeat (instantiate (1 := fun _ => True)).
+  unfold cache_inv_Property; intuition.
+  Grab Existential Variables.
+  exact (@weq _).
+  exact (@weq _).
+  exact (@weq _).
+  exact (@weq _).
+  exact Peano_dec.eq_nat_dec.
+Defined.
