src/BinEncoders/Env/Common/ComposeCheckSum.v
@@ -1,7 +1,8 @@
 Require Import
         Fiat.Computation
         Fiat.BinEncoders.Env.Common.Specs
-        Fiat.BinEncoders.Env.Common.Notations.
+        Fiat.BinEncoders.Env.Common.Notations
+        Fiat.BinEncoders.Env.Common.ComposeOpt.
 
 Section Checksum.
 
@@ -33,7 +34,7 @@ Section Checksum.
     `(q, ctx) <- encode2 ctx;
       ret (transform p (transform (calculate_checksum (transform p q)) q), ctx)%comp.
 
-  Lemma compose_encode_correct
+  Lemma composeChecksum_encode_correct
         {A'}
         {P  : CacheDecode -> Prop}
         {P_inv1 P_inv2 : (CacheDecode -> Prop) -> Prop}
@@ -111,10 +112,10 @@ Section Checksum.
              x3 = calculate_checksum (transform x x1))
     : encode_decode_correct_f
         cache transformer
-        (fun a => predicate a)
+        predicate
         predicate_rest'
-        (fun (data : A) (ctx : CacheEncode) =>
-           composeChecksum (encode1 (project data)) (encode2 data)  ctx
+        (fun (data : A) =>
+           composeChecksum (encode1 (project data)) (encode2 data)
         )%comp
         (fun (bin : B) (env : CacheDecode) =>
            if checksum_Valid_dec (encoded_A_measure bin) bin then
@@ -168,6 +169,153 @@ Section Checksum.
         simpl; eapply decodeChecksum_pf' in Heqo; intuition eauto.
     }
   Qed.
+
+  (* Corollary composeChecksum_compose_encode_correct *)
+  (*       {A_fst} *)
+  (*       {P  : CacheDecode -> Prop} *)
+  (*       {P_inv_fst P_inv_snd P_inv2 : (CacheDecode -> Prop) -> Prop} *)
+  (*       (decodeChecksum : B -> CacheDecode -> option (unit * B * CacheDecode)) *)
+  (*       (P_inv_pf : *)
+  (*          cache_inv_Property P (fun P => *)
+  (*                                  P_inv_fst P /\ P_inv_snd P /\ P_inv2 P *)
+  (*                                  /\ (forall b ctx u b' ctx', *)
+  (*                                         decodeChecksum b ctx = Some (u, b', ctx') *)
+  (*                                         -> P ctx *)
+  (*                                         -> P ctx'))) *)
+  (*       (project_fst : A -> A_fst) *)
+  (*       (project_snd : A -> A_snd) *)
+  (*       (predicate : A -> Prop) *)
+  (*       (predicate_fst : A_fst -> Prop) *)
+  (*       (predicate_snd : A_snd -> Prop) *)
+  (*       (predicate_rest' : A -> B -> Prop) *)
+  (*       (predicate_rest_fst : A_fst -> B -> Prop) *)
+  (*       (predicate_rest_snd : A_snd -> B -> Prop) *)
+  (*       (encode_fst : A_fst -> CacheEncode -> Comp (B * CacheEncode)) *)
+  (*       (encode_snd : A -> CacheEncode -> Comp (B * CacheEncode)) *)
+  (*       (encode2 : A -> CacheEncode -> Comp (B * CacheEncode)) *)
+  (*       (encoded_A_measure : B -> nat) *)
+  (*       (encoded_A_measure_OK : *)
+  (*          forall a ctx ctx' b ext, *)
+  (*            computes_to (composeChecksum (compose _ (encode_fst (project_fst a)) (encode_snd (project_snd a))) (encode2 a) ctx) (b, ctx') *)
+  (*            -> bin_measure b = encoded_A_measure (transform b ext)) *)
+  (*       (decode_fst : B -> CacheDecode -> option (A_fst * B * CacheDecode)) *)
+  (*       (decode_fst_pf : *)
+  (*          cache_inv_Property P P_inv_fst *)
+  (*          -> encode_decode_correct_f *)
+  (*               cache transformer predicate_fst *)
+  (*               predicate_rest_fst *)
+  (*               encode_fst decode_fst P) *)
+  (*       (pred_fst_pf : forall data, predicate data -> predicate_fst (project_fst data)) *)
+  (*       (*predicate_rest_impl : *)
+  (*          forall a' b *)
+  (*                 a ce ce' ce'' b' b'', *)
+  (*            computes_to (encode1 a' ce) (b', ce') *)
+  (*            -> project a = a' *)
+  (*            -> predicate a *)
+  (*            -> computes_to (encode2 a ce') (b'', ce'') *)
+  (*            -> predicate_rest' a b *)
+  (*            -> predicate_rest_fst a' (transform (transform (calculate_checksum (transform b' b'')) b'') b) *) *)
+  (*       (*decodeChecksum_pf : forall b b' ext a' ctx ctx' ctxD, *)
+  (*           computes_to (encode1 a' ctx) (b, ctx') *)
+  (*           -> Equiv ctx' ctxD *)
+  (*           -> decodeChecksum (transform (transform (calculate_checksum (transform b b')) b') ext) ctxD = *)
+  (*              Some (tt, transform b' ext, ctxD)) *)
+  (*       (decodeChecksum_pf' : forall u b b' ctx ctxD ctxD', *)
+  (*           Equiv ctx ctxD *)
+  (*           -> decodeChecksum b ctxD = Some (u, b', ctxD') *)
+  (*           -> Equiv ctx ctxD' *)
+  (*              /\ exists b'', b = transform b'' b'*) *)
+  (*       (decode2 : A_fst -> B -> CacheDecode -> option (A * B * CacheDecode)) *)
+  (*       (decode2_pf : forall proj_fst proj_snd, *)
+  (*           predicate_fst proj_fst -> *)
+  (*           predicate_snd proj_snd -> *)
+  (*           cache_inv_Property P P_inv2 -> *)
+  (*           encode_decode_correct_f cache transformer *)
+  (*                                   (fun data => predicate data *)
+  (*                                                /\ project_fst data = proj_fst *)
+  (*                                                /\ project_snd data = proj_snd) *)
+  (*                                   predicate_rest' *)
+  (*                                   encode2 *)
+  (*                                   (decode2 proj_fst proj_snd) P) *)
+  (*       (*checksum_Valid_chk : *)
+  (*          forall env env' xenv' data ext c0 c1 x x0 x1 x2 x3, *)
+  (*            Equiv env env' -> *)
+  (*            P env' -> *)
+  (*            Equiv x0 c0 -> *)
+  (*            P xenv' -> *)
+  (*            Equiv x2 xenv' -> *)
+  (*            predicate data -> *)
+  (*            encode_decode_correct_f cache transformer predicate' predicate_rest encode1 decode1 P -> *)
+  (*            encode1 (project data) env ↝ (x, x0) -> *)
+  (*            predicate' (project data) -> *)
+  (*            decode2 (project_fst data) (transform x1 ext) c1 = Some (data, ext, xenv') -> *)
+  (*            encode2 data x0 ↝ (x1, x2) -> *)
+  (*            Equiv x0 c1 -> *)
+  (*            checksum_Valid (encoded_A_measure (transform x (transform x3 (transform x1 ext)))) (transform x (transform x3 (transform x1 ext))) -> *)
+  (*            x3 = calculate_checksum (transform x x1)*) *)
+  (*   : encode_decode_correct_f *)
+  (*       cache transformer *)
+  (*       (fun a => predicate a) *)
+  (*       predicate_rest' *)
+  (*       (fun (data : A) (ctx : CacheEncode) => *)
+  (*          composeChecksum (compose _ (encode_fst (project_fst data)) (encode_snd (project_snd data))) (encode2 data)  ctx *)
+  (*       )%comp *)
+  (*       (fun (bin : B) (env : CacheDecode) => *)
+  (*          if checksum_Valid_dec (encoded_A_measure bin) bin then *)
+  (*            `(proj_fst, rest, env') <- decode_fst bin env; *)
+  (*            `(proj_snd, rest, env') <- decode_snd rest env'; *)
+  (*            `(_, rest', env') <- decodeChecksum rest env'; *)
+  (*              decode2 proj_fst proj_snd rest' env' *)
+  (*          else None) *)
+  (*       P. *)
+  (* Proof. *)
+  (* Admitted. *)
+  (*unfold cache_inv_Property in *; split.
+    { intros env env' xenv data bin ext env_pm pred_pm pred_pm_rest com_pf.
+      eapply composeChecksum_encode_correct in com_pf.
+
+      unfold composeChecksum, Bind2 in com_pf; computes_to_inv; destruct v;
+        destruct v0.
+      destruct (fun H' => proj1 (decode1_pf (proj1 P_inv_pf)) _ _ _ _ _ (transform (transform (calculate_checksum (transform b b0)) b0) ext) env_pm (pred_pf _ pred_pm) H' com_pf); intuition; simpl in *; injections; eauto.
+      find_if_inside.
+      - setoid_rewrite <- transform_assoc; rewrite H2.
+        simpl; rewrite (decodeChecksum_pf _ _ _ _ _ _ _ com_pf); simpl; eauto.
+        destruct (fun H'' => proj1 (decode2_pf (project data) (pred_pf _ pred_pm) H)
+                                   _ _ _ _ _ ext H3 (conj pred_pm (eq_refl _)) H'' com_pf');
+          intuition; simpl in *; injections.
+        eauto.
+      - destruct f.
+        erewrite <- encoded_A_measure_OK, <- transform_assoc, checksum_commute; eauto.
+        rewrite !transform_assoc.
+        rewrite checksum_Valid_commute, transform_assoc; eauto.
+        computes_to_econstructor; eauto.
+        computes_to_econstructor; eauto.
+    }
+    { intros.
+      find_if_inside; try discriminate.
+      - destruct (decode1 bin env') as [ [ [? ?] ? ] | ] eqn : ? ;
+          simpl in *; try discriminate.
+        eapply (proj2 (decode1_pf (proj1 P_inv_pf))) in Heqo; eauto.
+        destruct Heqo as [? [? [? [? [? [? ?] ] ] ] ] ]; subst.
+        destruct (decodeChecksum b c0) as [ [ [? ?] ? ] | ] eqn : ? ;
+          simpl in *; try discriminate.
+        eapply P_inv_pf in H2; eauto.
+        eapply (proj2 (decode2_pf a H5 (proj1 (proj2 P_inv_pf)))) in H2; eauto.
+        destruct H2 as [? ?]; destruct_ex; intuition; subst.
+        eexists; eexists; repeat split.
+        repeat computes_to_econstructor; eauto.
+        simpl; rewrite transform_assoc.
+        rewrite <- !transform_assoc.
+        eapply decodeChecksum_pf' in Heqo; eauto; intuition; destruct_ex;
+          subst.
+        simpl in *.
+        repeat f_equal.
+        eauto.
+        eassumption.
+        simpl; eassumption.
+        simpl; eapply decodeChecksum_pf' in Heqo; intuition eauto.
+    }
+  Qed. *)
 
 End Checksum.
 
